\documentclass[a4paper]{article}
\usepackage{amssymb, amsmath}
\usepackage{graphicx}
\begin{document}
\section{Gaussian Random Number Generator}
Given $U_1$ and $U_2$ belong $[-1,1]$, the following is to find out random variables that are Gaussian distributed.\\

\noindent{\bf a. Principle}\\
1)	Start from an cdf of joint Gaussian random variable x and y\\
\begin{align*}
& \int \int exp(-1/2 x^2)  exp(-1/2 y^2)  dx dy \\
 = & \int d \theta \int r exp(-r^2/2) dr\\
 = & \int pdf(\theta) * \int pdf(r)\\
\end{align*}
So if we are able to fine r and $\theta$, then by taking x = r cos $\theta$, y = r sin $\theta$, we get x and y\\
2)	To fine $\theta$ is easy as we can take $\theta = 2 \pi U_2$\\
3)	Suppose $R = \sqrt{-2 ln U_1}$\\
The cdf of R is
\begin{align*}
& P(R <= r) \\
 = &P(\sqrt{-2 U_1} <= r) \\
 = &P(U_1 >= exp(-1/2 r^2)) \\
 = &\int_{exp(1/2r^2)}^1 du_1 \\
 = &1 - exp(-1/2 r^2)	\\
\end{align*}

So the $pdf = r exp(-1/2 r^2)$\\
4)	Therefore
\begin{align*}
X = \sqrt{-2 ln U_1} cos(2\pi U_2) \\
Y = \sqrt{-2 ln U_1} sin(2\pi U_2) \\
\end{align*}

\noindent{\bf b.	Efficient way of evaluating cos and sin function} \\
In most computers, evaluating cos and sine is not quite straightforward, so the above method is not practical to use. So the following alternative avoids evaluating sine and cos functions directly.\\
1)	We generate new random variable $S = U_1^2 + U_2^2$
\begin{align*}
 P(S<s) &= P(U_1^2 + U_2^2 <s) \\
& = \int\int_{u_1^2 + u_2^2} 1 dx dy\\
& = \int_0 ^{\sqrt{s}} r dr *2\pi \\
& = \pi r^2|_0^s \\
& = \pi s \\
\end{align*}
So pdf of s is 1/pi, it is uniform distribution.\\
2)	Now if we let $S<1$, by taking S that satisfies only $U_1^2 + U_2^2 <1$, then throwing away others, then S is uniform in (0,$\pi$), which corresponds r in(0, 1)\\
Then a.4) becomes\\
\begin{align*}
X = \sqrt{-2 ln S} cos(2\pi S) =\sqrt{-2 ln S} U_1/\sqrt{S} \\
Y = \sqrt{-2 ln S} sin(2\pi S) = \sqrt{-2 ln S} U_2/\sqrt{S} \\
\end{align*}


{\bf c.	Final algorithm} \\
1)	Generate two uniform random variables $U_1$ $U_2$ y belongs to [-1, 1]\\
2)	If $U_1^2 + U_2^2 >=1$, throw away and regenerate.\\
3)	Return\\ 
\begin{align*}
    U_1 * \sqrt{-2 log (U_1^2 + U_2^2) / (U_1^2 + U_2 ^2)}\\
    U_2 * \sqrt{-2 log (U_1^2 + U_2^2) / (U_1^2 + U_2 ^2)}\\
\end{align*}







\end{document}