\documentclass[a4paper]{article}
\usepackage{amssymb, amsmath}
\usepackage{graphicx}
\begin{document}
\section{Ito Integral}


\noindent{ \bf a. Ito Integral Definition for simple integrand}\\
Given $t_0$, $t_1$бн $t_n$ and $\Delta t$ is a constant in between any $[t_k, t_{k+1}]$\\
\begin{align*}
I(t) = \sum_{j=0}^{k-1} \Delta(t_j)[W(t_{j+1}) - W(t_{j}) ]
         + \Delta(t_k)[W(t) - W(t_k)]        	
\end{align*}
We can also rewrite $I(t) = \int_0 ^t \Delta(u) dW(u)$.\\
 
\noindent{ \bf b. Properties of Ito integral} \\
1)	Ito Integral is a martingale \\
2)	Isometry \\
$E I^2(t) = E \int_0 ^t \Delta^2(u) du$ \\

\noindent{ \bf c. Ito integral definition for general integrand } \\
Choose $\Delta_n(t)$ such that when $n-> \infty$ \\
$lim_{n->\infty} E \int_0 ^T |\Delta_n(t) -\Delta(t)|^2 dt =0$ \\
Define Ito integral\\
\begin{align*}
	\int_0^t \Delta(u) dW(u) = lim_{n->\infty} \int_0^t \Delta_n(u) dW(u)
\end{align*}

\section{Ito formula }
\noindent{\bf a. Ito formula}
Suppose 
$dX_t = u dt + \sigma dB_t$ \\
If g(t, X) is twice continuously differentiable   $Y_t = g(t, X_t)$ \\
\begin{align*}
	d Y_t = \frac{\partial g}{\partial t} dt + \frac{\partial g}{\partial X} dX_t \\
          + \frac{1}{2} \frac{\partial^2 g}{\partial x^2} (d X_t)^2
\end{align*}
Where $(dX)^2 = d(X_t) d(X_t) = u^2 (dt)^2 + 2 u \sigma dt dB_t
                                                       + \sigma^2 (dB_t)^2$\\
$dt * dt = dt * dB_t = 0$, $dB_t dB_t = dt$ \\
So $(d X_t)^2 = \sigma^2 dt$. \\

\noindent {\bf b. Example: Geometric Brownian motion}\\
The geometric Brownian motion satisfies
$d N_t /N_t= r  dt + \sigma dB_t$
to solve this we consider\\
\begin{align*}
	d(ln N_t)
&= \frac{\partial ln N_t}{\partial N_t} d N_t 
+\frac{1}{2} \frac{\partial^2  ln N_t}{ \partial N_t ^2} (dN_t)^2 \\
&= \frac{1}{N_t} d N_t + \frac{1}{2} (-\frac{1}{N_t^2}) (d N_t)^2 \\
(d N_t)^2 &= r^2 N_t ^2 (dt)^2 + r N_t dt \sigma d B_t 
+ \sigma^2 N_t^2 d^2 B_t \\
                  & = 0 + 0 +  \sigma^2 N_t^2 dt \\
\end{align*}
So   
\begin{align*}
d(ln N_t) = \frac{1}{N_t} d N_t  - \frac{1}{2}\sigma^2 dt
                        = (r - \frac{1}{2} \sigma^2 ) dt + \sigma d B_t\\	
ln (N_t/ N_0) =  (r - \frac{1}{2} \sigma^2 ) t + \sigma  B_t \\
N_t =  N_0 exp(   (r - \frac{1}{2} \sigma^2 ) t + \sigma  B_t) \\
\end{align*}

\end{document}