\documentclass[a4paper]{article}
\usepackage{amssymb, amsmath}
\usepackage{graphicx}
\begin{document}
\section{Random Walk}
\subsection{Symmetric Random Walk}
\subsubsection{Definition}
Starting from coin toss, \\
def:
\begin{align*}
X_j & =  1 \hspace{2mm} &if \hspace{2mm} w_j = H\\
    & = -1 \hspace{2mm} &if \hspace{2mm} w_j = T	
\end{align*}
Let $M_k = \sum_{j=1} ^{k} X_j$, $M_k$ is symmetric random walk, and its distribution is binomial.\\

\subsubsection{Expectation and Variance}
$E(X_j) =0$, $Var(X_j) =1$,\\
$Var(M_k - M_l) = \sum_{i=l}^{k} Var(X_i) = k - l$;\\

\subsubsection{Martingale Property} 
$E(M_l| F_k)$\\
$=E((M_l - M_k + M_k) | F_k)$\\
$=E((M_l - M_k) | F_k) + E(M_k | F_k)$\\
$=0 + M_k = M_k$\\

\subsection{Scaled Random Walk}
\subsubsection{Scaled Symmetric Random Walk Definition}
\begin{align*}
W^{(n)}(t) = 1/\sqrt{n} M_{nt}  \\
= 1/\sqrt{n} \sum_{i=1}^{nt} X^{(n)}(t)\\
= \sum_{i=1} ^{nt}  1/\sqrt{n} X^{(n)}(t) \\
\end{align*}
\subsubsection{Expectation and Variance}
\begin{align*}
E(W^{(n)}(t) - W^{(n)}(s)) =0 \\
Var(W^{(n)}(t) - W^{(n)}(s)) = n(t-s) Var(1/\sqrt{n} X^{(n)} (t-s) )
=t - s
\end{align*}


\subsection{Brownian Motion}
\subsubsection{Limit of Scaled Symmetric Random Walk: Brownian Motion} 
When $n-> \inf$, based on Central Limit Theorem\\ 
$W^{(n)}(t)$ starting from 0 follows a normal distribution N(0, t)\\
We view $W^{(n)}(t)$ as a Brownian motion\\

\subsubsection {Quadratic variation of Brownian motion }
 Given a Brownian motion $W_{t_j}$
 Define 
 \begin{align*}
	Q &= \sum_{j=0} ^{n-1} (W_{t_{j+1}} - W_{t_j})^2 \\
 	E(Q)  &= \sum_{j=0} ^{n-1} E ((W_{t_{j+1}} - W_{t_j})^2) \\
       & = \sum_{j=0} ^{n-1} (t_{j+1} - t_j) \\
       & = T
\end{align*}

 \begin{align*}
   Var(Q) = \sum_{j=0}^{n-1} 2(t_{j+1} - t_{j})^2 \\
   <= 2|C|T (where ||C|| = max|t_{j+1} - t_{j} |) \\
    When |C| = 0, \\
    Var(Q) = 0 \\
 \end{align*}
This is simply written in differential form $dW dW$ = $dt$\\

\subsubsection{From Scaled Asymmetric Random Walk to Geometric Brownian motion}

Consider a scaled asymmetric random walk with factor of $\sigma$ and drift $\alpha$
  \begin{align*}
	W^{(n)}(t) =  \sigma  (\frac{1}{\sqrt{n}} M_{nt} )+ \alpha t
  \end{align*}
  
  Construct new random variable which satisfies
  $\delta S / S = W^{(n)}(t)$ , which is equivalent to 
	
	\begin{align*}
  S+ = S(1+\alpha /n + \sigma /\sqrt{n}) \\
  S- =  S(1+\alpha /n - \sigma /\sqrt{n}) \\
	\end{align*}
  Assuming number of heads is $H_{nt}$, number of tails is $T_{nt}$
  Then 
  \begin{align*}
	 S_n(t) &= S_n(0) (1+\alpha /n + \sigma /\sqrt{n})^{(H_{nt})} (1+\alpha /n - \sigma /\sqrt{n})^{(T_{nt})} \\
   \end{align*}
 
 \begin{align*}
	log(S_n(t)) & = log(S_n(0)) + (H_{nt}) log(1+\alpha /n + \sigma /\sqrt{n})
								+ (T_{nt}) log(1+\alpha /n - \sigma /\sqrt{n})\\
				& = log(S_n(0)) + (H_{nt}) (\alpha /n + \sigma /\sqrt{n} - 1/2(\alpha /n + \sigma /\sqrt{n})^2)\\
				& +(T_{nt}) (\alpha /n - \sigma /\sqrt{n} - 1/2(\alpha /n - \sigma /\sqrt{n})^2)\\
				& = log(S_n(0)) +(H_{nt} + T_{nt}) (\alpha/n - \sigma^2 /n + O(n^{-3/2}))
				+ (H_{nt} - T_{nt}) (\sigma /\sqrt{n} )\\
				& = log(S_n(0)) + nt(\alpha /n - 1/2 \sigma^2 /n) + M_{nt} \sigma/\sqrt{n}\\
				& = log(S_n(0)) + (\alpha - \frac{1}{2} \sigma^2)t + W^{n}(t) \sigma \\
\end{align*}
  Then we can prove when $n-> \infty$
  The distribution of $S_n(t)$ converges to the distribution of
  \begin{align*}
	  S(t) = S(0) exp((\alpha - \frac{1}{2} \sigma^2 )t +\sigma W(t))
  \end{align*}
  Where W(t) is a normal random variable with mean 0 and variance t. 








\end{document}
